theories/stlc/Triangular.v
@@ -99,8 +99,20 @@ Module Tri.
   #[global] Arguments refl {_}.
   #[global] Arguments cons {_ _} x {_} t ζ.
 
+  #[export] Instance InstTri : forall w, Inst (Tri w) (Assignment w) :=
+    fix insttri {w0 w1} (r : Tri w0 w1) :=
+      match r with
+      | Tri.refl => fun ι => ι
+      | @Tri.cons _ w' x xIn t r =>
+          fun ι =>
+            let ι' := inst (Inst := @insttri _) r ι in
+            env.insert xIn ι' (inst t ι')
+      end.
+
   #[export] Instance refl_tri : Refl Tri :=
     fun w => refl.
+  #[export] Instance instrefl_tri : InstRefl Tri :=
+    fun _ _ => eq_refl.
   #[export] Instance trans_tri : Trans Tri :=
     fix trans [w0 w1 w2] (ζ1 : w0 ⊒⁻ w1) {struct ζ1} : w1 ⊒⁻ w2 -> w0 ⊒⁻ w2 :=
       match ζ1 with
@@ -145,15 +157,6 @@ fix F (w c : World) (t : w ⊒⁻ c) {struct t} : P w c t :=
     - induction r1; cbn; congruence.
   Qed.
 
-  #[export] Instance InstTri : forall w, Inst (Tri w) (Assignment w) :=
-    fix insttri {w0 w1} (r : Tri w0 w1) :=
-      match r with
-      | Tri.refl => fun ι => ι
-      | @Tri.cons _ w' x xIn t r =>
-          fun ι =>
-            let ι' := inst (Inst := @insttri _) r ι in
-            env.insert xIn ι' (inst t ι')
-      end.
 
   Definition single {w} x {xIn : x ∈ w} (t : Ty (w - x)) : w ⊒⁻ w - x :=
     cons x t refl.
